solved problems 1-4

problems/4/Problem4.dfy
@@ -1,9 +1,66 @@
+include "../../parser/split.dfy"
+include "../../parser/parseInt.dfy"
+include "../../libraries/src/dafny/Collections/Seqs.dfy"
 module Problem4 {
+    import opened Split
+    import opened ParseInt
+    import opened Dafny.Collections.Seq
+
+    predicate Increasing(xs: seq<int>) {
+        forall i :: 0 <= i < |xs|-1 ==> xs[i] <= xs[i+1]
+    }    
+
+    predicate Inc(xs: seq<int>) {
+        if |xs| > 1 then xs[0] <= xs[1] && Inc(xs[1..]) else true
+    }
+
+    predicate LastNotZer0(xs: seq<int>) {
+        if |xs| > 1 then xs[|xs|-1] >= xs[|xs|-2] else false
+    }
+
+    predicate DuplicateExists(xs: seq<int>) {
+        exists i :: 0 <= i < |xs|-1 && xs[i] == xs[i+1] &&  (0 <= i - 1 ==> xs[i-1] != xs[i]) && (i+2 < |xs| ==> xs[i+2] != xs[i])
+    }
+
+    predicate HasDuplicate(xs: seq<int>) {
+        if |xs| > 1 then xs[0] == xs[1] || HasDuplicate(xs[1..]) else false
+    }
+
     method problem4_1(input: string) returns (x: int) {
-        return 3;
+        var pieces := Map(Integer, split(input,"-"));
+        assume {:axiom} |pieces| == 2 && pieces[0] <= pieces[1];
+        x := 0;
+        // assert !Inc([7,7,7,7,7,0]);
+        for i := pieces[0] to pieces[1] {
+            var numString := toStr(i);
+            var nums := Map(Integer, split(numString, ""));
+            if Increasing(nums) && HasDuplicate(nums)  {
+                print i,"\n";
+                print "numString", numString, "\n";
+                print "nums ", nums, "\n";
+                x := x +1;
+            }
+        }
     }
 
     method problem4_2(input: string) returns (x: int) {
-        return 4;
+        var pieces := Map(Integer, split(input,"-"));
+        assume {:axiom} |pieces| == 2 && pieces[0] <= pieces[1];
+        x := 0;
+        // assert !Inc([7,7,7,7,7,0]);
+        expect DuplicateExists([1,1,1,1,2,2]);
+        expect DuplicateExists([1,1,2,2,3,3]);
+        expect !DuplicateExists([1,2,3,4,4,4]);
+        expect DuplicateExists([3,3,4,5,6,7]);
+        for i := pieces[0] to pieces[1] {
+            var numString := toStr(i);
+            var nums := Map(Integer, split(numString, ""));
+            if Increasing(nums) && DuplicateExists(nums)  {
+                print i,"\n";
+                print "numString", numString, "\n";
+                print "nums ", nums, "\n";
+                x := x +1;
+            }
+        }
     }
 }
