problems/1/Problem1.dfy
@@ -2,14 +2,39 @@ include "../../parser/split.dfy"
 include "../../parser/parseInt.dfy"
 include "../../libraries/src/dafny/Collections/Seqs.dfy"
 module Problem1 {
+    import opened Split
+    import opened ParseInt
+    import opened Dafny.Collections.Seq
+    
+    method parseInput(input: string) returns (s: seq<int>) {
+        var res := splitOnBreak(input);
+        s := Map(xs => Integer(xs), Filter(xs => xs != "", res));
+    }
+
+    function sum(s: seq<int>): int {
+        if |s| == 0 then 0 else s[0] + sum(s[1..])
+    }
+
+    function calcFuel(x: int): int {
+        (x/3)-2
+    }
+
+    function recCaclFuel(x: int, partialSum: int): int {
+        var fuel := calcFuel(x);
+        if fuel > 0 then recCaclFuel(fuel, partialSum + fuel) else partialSum
+    }
 
     method problem1_1(input: string) returns (x: int)
     {
-        return 1;
+        var data := parseInput(input);
+        return sum(Map(calcFuel, data));
     }
 
     method problem1_2(input: string) returns (x: int)
     {
-        return 2;
+        var data := parseInput(input);
+        var partial := Map(x => recCaclFuel(x,0), data);
+        print partial;
+        return sum(partial);
     }
 }
