problems/2/Problem2.dfy
@@ -1,9 +1,88 @@
+include "../../parser/split.dfy"
+include "../../parser/parseInt.dfy"
+include "../../libraries/src/dafny/Collections/Seqs.dfy"
 module Problem2 {
+    import opened Split
+    import opened ParseInt
+    import opened Dafny.Collections.Seq
+    method parseInput(input: string) returns (s: seq<int>) {
+        var res := Split.split(input, ",");
+        s := Map(Integer, res);
+    }
+
+    method executeIntcodes(intcodes: array<int>) 
+        modifies intcodes
+        requires intcodes.Length > 0
+    {
+        var i:=0;
+        // print "here";
+        while i < intcodes.Length {
+            match intcodes[i] {
+                case 1 => {
+                    assume {:axiom} i+4 < intcodes.Length;
+                    var pos1 := intcodes[i+1];
+                    var pos2 := intcodes[i+2];
+                    var dest := intcodes[i+3];
+                    assume {:axiom} 0 <= pos1 < intcodes.Length;
+                    assume {:axiom} 0 <= pos2 < intcodes.Length;
+                    assume {:axiom} 0 <= dest < intcodes.Length;
+                    intcodes[dest]:=intcodes[pos1]+intcodes[pos2];
+                    i := i + 4;
+                }
+                case 2 => {
+                    assume {:axiom} i+4 < intcodes.Length;
+                    var pos1 := intcodes[i+1];
+                    var pos2 := intcodes[i+2];
+                    var dest := intcodes[i+3];
+                    assume {:axiom} 0 <= pos1 < intcodes.Length;
+                    assume {:axiom} 0 <= pos2 < intcodes.Length;
+                    assume {:axiom} 0 <= dest < intcodes.Length;
+                    intcodes[dest]:=intcodes[pos1]*intcodes[pos2];
+                    i := i + 4;
+                }
+                case 99 => {
+                    break;
+                }
+                case _ => {
+                    print "Error: encounted bad incode", intcodes[i], i, "\n";
+                    break;
+                }
+            }
+        }
+    }
+
     method problem2_1(input: string) returns (x: int) {
-        return 3;
+        var data:= parseInput(input);
+        assume {:axiom} |data| > 3;
+        print data, "\n"; 
+        var arr := ToArray(data);
+        arr[1]:=12;
+        arr[2]:=2;
+        executeIntcodes(arr);
+        return arr[0];
     }
 
     method problem2_2(input: string) returns (x: int) {
-        return 4;
+        var data:= parseInput(input);
+        assume {:axiom} |data| > 3;
+        print data, "\n"; 
+        var noun := 0;
+        while noun <= 99 {
+            var verb := 0;
+            while verb <= 99 {
+
+                var arr := ToArray(data);
+                arr[1]:=noun;
+                arr[2]:=verb;
+                executeIntcodes(arr);
+                if arr[0] == 19690720 {
+                    // print "got here", noun, verb;
+                    return 100*noun + verb;
+                }
+                verb := verb + 1;
+            }
+            noun := noun + 1;
+        }
+        x := -1;
     }
 }
