problems/3/Problem3.dfy
@@ -1,9 +1,146 @@
+include "../../parser/split.dfy"
+include "../../parser/parseInt.dfy"
+include "../../libraries/src/dafny/Collections/Seqs.dfy"
+include "../../parser/regex.dfy"
 module Problem3 {
-    method problem3_1(input: string) returns (x: int) {
-        return 3;
+    import opened Split
+    import opened ParseInt
+    import opened Dafny.Collections.Seq
+    import opened RegEx
+    datatype Direction = Up | Right | Down | Left
+    datatype Step = Step(step: nat, dir: Direction)
+    datatype Point = Point(x: int, y: int)
+    function abs(x: int): nat {
+        if x < 0 then -x else x
     }
 
-    method problem3_2(input: string) returns (x: int) {
-        return 4;
+    function manhattanDist(p1: Point, p2: Point): int {
+        abs(p1.x-p2.x) + abs(p1.y-p2.y)
+    }
+
+    method parseInput(input: string) returns (s: seq<seq<Step>>)
+        decreases * 
+    {
+        s := [];
+        var lines := Filter(x => x != "", splitOnBreak(input));
+        for i := 0 to |lines| {
+            var stepsStrings := split(lines[i],",");
+            var steps: seq<Step> := [];
+            for k := 0 to |stepsStrings| {
+
+                var matches, captures := ReMatch("(U|R|D|L)((1|2|3|4|5|6|7|8|9|0)+)", stepsStrings[k]);
+                expect matches;
+                assume {:axiom} |captures| == 3;
+                var step := match captures[1] {
+                    case "U" => Step(abs(Integer(captures[2])), Up)
+                    case "R" => Step(abs(Integer(captures[2])), Right)
+                    case "L" => Step(abs(Integer(captures[2])), Left)
+                    case "D" => Step(abs(Integer(captures[2])), Down)
+                    case _ => Step(0, Down)
+                };
+                steps := steps + [step];
+            }
+            s := s + [steps];
+        }
+    }
+
+    function step(d: Direction, p: Point): Point {
+        match d {
+            case Up => Point(p.x, p.y+1)
+            case Down => Point(p.x, p.y-1)
+            case Left => Point(p.x-1, p.y)
+            case Right => Point(p.x+1, p.y)
+        }
+    }
+
+    method findNearest(data: seq<seq<Step>>) returns (x: int)
+
+    {
+        var linePoints : set<Point> := {};
+        var intersections: set<Point> := {};
+        for i := 0 to |data| {
+            var pos := Point(0,0);
+            for k := 0 to |data[i]| {
+                for j:= 0 to data[i][k].step {
+                    pos := step(data[i][k].dir, pos);
+                    if i == 0 {
+                        linePoints := linePoints + {pos};
+                    }else{
+                        if pos in linePoints {
+                            intersections := intersections + {pos};
+                        }
+                    }
+                }
+            }
+        }
+        var origin := Point(0,0);
+        var d := -1;
+        print intersections;
+        while intersections != {} {
+            var px :| px in intersections;
+            var distance := manhattanDist(px, origin);
+            if d == -1 {
+                d := distance;
+            }else if distance < d {
+                d := distance;
+            }
+            intersections := intersections - {px};
+        }
+        return abs(d);
+    }
+
+    method findFastest(data: seq<seq<Step>>) returns (x: int)
+
+    {
+        var linePoints : set<Point> := {};
+        var pointDist : map<Point, nat> := map[];
+        var intersections: set<nat> := {};
+        for i := 0 to |data| {
+            var pos := Point(0,0);
+            var dist := 0;
+            for k := 0 to |data[i]| {
+                for j:= 0 to data[i][k].step {
+                    pos := step(data[i][k].dir, pos);
+                    dist := dist + 1;
+                    if i == 0 {
+                        linePoints := linePoints + {pos};
+                        pointDist := pointDist[pos := dist];
+                    }else{
+                        if pos in linePoints && pos in pointDist {
+                            intersections := intersections + {dist+pointDist[pos]};
+                        }
+                    }
+                }
+            }
+        }
+        var origin := Point(0,0);
+        var d: int := -1;
+        print intersections;
+        while intersections != {} {
+            var px :| px in intersections;
+            if d == -1 || px < d {
+                d := px;
+            }
+            intersections := intersections - {px};
+        }
+        return abs(d);
+    }
+
+    method problem3_1(input: string) returns (x: int)
+        decreases *
+    {
+        var data := parseInput(input);
+        // print data;
+        var dist := findNearest(data);
+        return dist;
+    }
+
+    method problem3_2(input: string) returns (x: int)
+        decreases *
+    {
+        var data := parseInput(input);
+        // print data;
+        var dist := findFastest(data);
+        return dist;
     }
 }
